test/new_treehash/test_new_version.c
@@ -14,7 +14,7 @@
 #include "xmss_core.h"
 
 #ifndef TESTS
-#define TESTS 10
+#define TESTS 1
 #endif
 
 static int starts_with(const char *str, const char *prefix) { return strncmp(str, prefix, strlen(prefix)) == 0; }
@@ -193,7 +193,7 @@ int main() {
     // char *impls[] = {"XMSS-SHA2_10_256", "XMSS-SHA2_10_192", "XMSSMT-SHA2_20/2_256", "XMSSMT-SHA2_20/4_256"};
     char *impls[] = {"XMSSMT-SHA2_20/2_256"};
 
-    size_t impl_count = 4;
+    size_t impl_count = 1; /* TODO: Update this */
 
     for (size_t i = 0; i < impl_count; i++) {
         if (starts_with(impls[i], "XMSSMT")) {
@@ -224,7 +224,7 @@ int main() {
         }
 
         test_kg(p);
-        test_sign(p);
+        // test_sign(p);
 
         if (debug) {
             puts("=====================================================================================");
